src/cbor/pulse/raw/CBOR.Pulse.Raw.Iterator.fst
@@ -1,6 +1,7 @@
 module CBOR.Pulse.Raw.Iterator
 #lang-pulse
 include CBOR.Pulse.Raw.Iterator.Base
+include CBOR.Pulse.Raw.Iterator.Gen
 open CBOR.Pulse.Raw.Util
 open Pulse.Lib.Pervasives
 open Pulse.Lib.Trade
@@ -391,33 +392,6 @@ let cbor_raw_iterator_match
   | CBOR_Raw_Iterator_Serialized c' -> ser_match pm c' l
 
 inline_for_extraction
-let cbor_raw_iterator_init_from_slice_t
-  (#cbor_raw_iterator: Type0)
-  (#elt_low #elt_high: Type0)
-  (elt_match: perm -> elt_low -> elt_high -> slprop)
-  (cbor_raw_iterator_match: perm -> cbor_raw_iterator -> list elt_high -> slprop)
-=
-  (a: S.slice elt_low) ->
-  (#pm: perm) ->
-  (#pm': perm) ->
-  (#l: Ghost.erased (list elt_high)) ->
-  (#sq: Ghost.erased (Seq.seq elt_low)) ->
-  stt cbor_raw_iterator
-  (requires
-  pts_to a #pm sq **
-  PM.seq_list_match sq l (elt_match pm') **
-  pure (FStar.UInt.fits (SZ.v (S.len a)) U64.n)
-  )
-  (ensures fun res -> exists* p .
-  cbor_raw_iterator_match p res l **
-     trade
-       (cbor_raw_iterator_match p res l)
-       (pts_to a #pm sq **
-         PM.seq_list_match sq l (elt_match pm')
-       )
-  )
-
-inline_for_extraction
 fn cbor_raw_iterator_init_from_slice
   (#elt_low #elt_high: Type0)
   (elt_match: perm -> elt_low -> elt_high -> slprop)
@@ -441,20 +415,22 @@ fn cbor_raw_iterator_init_from_slice
 }
 
 inline_for_extraction
-let cbor_raw_iterator_is_empty_t
-  (#elt_high #cbor_raw_iterator: Type0)
-  (cbor_raw_iterator_match: perm -> cbor_raw_iterator -> list elt_high -> slprop)
-= (c: cbor_raw_iterator) ->
-  (#pm: perm) ->
-  (#r: Ghost.erased (list elt_high)) ->
-  stt bool
-  (requires
-    cbor_raw_iterator_match pm c r
-  )
-  (ensures fun res ->
-    cbor_raw_iterator_match pm c r **
-    pure (res == Nil? r)
-  )
+fn cbor_raw_iterator_init_from_serialized
+  (#elt_low #elt_high: Type0)
+  (elt_match: perm -> elt_low -> elt_high -> slprop)
+  (ser_match: perm -> cbor_raw_serialized_iterator -> list elt_high -> slprop)
+: cbor_raw_iterator_init_from_serialized_t #_ #_ #_ ser_match (cbor_raw_iterator_match elt_match ser_match)
+=
+  (a: cbor_raw_serialized_iterator)
+  (#pm: perm)
+  (#l: Ghost.erased (list elt_high))
+{
+  let res : cbor_raw_iterator elt_low = CBOR_Raw_Iterator_Serialized a;
+  Trade.rewrite_with_trade
+    (ser_match pm a l)
+    (cbor_raw_iterator_match elt_match ser_match pm res l);
+  res
+}
 
 inline_for_extraction
 let cbor_raw_serialized_iterator_is_empty_t
@@ -495,23 +471,6 @@ fn cbor_raw_iterator_is_empty
 }
 
 inline_for_extraction
-let cbor_raw_iterator_length_t
-  (#elt_high #cbor_raw_iterator: Type0)
-  (cbor_raw_iterator_match: perm -> cbor_raw_iterator -> list elt_high -> slprop)
-=
-  (c: cbor_raw_iterator) ->
-  (#pm: perm) ->
-  (#r: Ghost.erased (list elt_high)) ->
-  stt U64.t
-  (requires
-    cbor_raw_iterator_match pm c r
-  )
-  (ensures fun res ->
-    cbor_raw_iterator_match pm c r **
-    pure ((U64.v res <: nat) == List.Tot.length r)
-  )
-
-inline_for_extraction
 let cbor_raw_serialized_iterator_length_t
   (#elt_high: Type0)
   (ser_match: perm -> cbor_raw_serialized_iterator -> list elt_high -> slprop)
@@ -548,33 +507,6 @@ fn cbor_raw_iterator_length
     }
   }
 }
-
-inline_for_extraction
-let cbor_raw_iterator_next_t
-  (#cbor_raw_iterator: Type0)
-  (#elt_low #elt_high: Type0)
-  (elt_match: perm -> elt_low -> elt_high -> slprop)
-  (cbor_raw_iterator_match: perm -> cbor_raw_iterator -> list elt_high -> slprop)
-=
-  (pi: R.ref (cbor_raw_iterator)) ->
-  (#pm: perm) ->
-  (#i: Ghost.erased cbor_raw_iterator) ->
-  (#l: Ghost.erased (list elt_high)) ->
-  stt elt_low
-  (
-    R.pts_to pi i **
-    cbor_raw_iterator_match pm i l **
-    pure (Cons? l)
-  )
-  (fun res -> exists* a p i' q .
-    elt_match p res a **
-    R.pts_to pi i' **
-    cbor_raw_iterator_match pm i' q **
-    trade
-      (elt_match p res a ** cbor_raw_iterator_match pm i' q)
-      (cbor_raw_iterator_match pm i l) **
-    pure (Ghost.reveal l == a :: q)
-  )
 
 inline_for_extraction
 let cbor_raw_serialized_iterator_next_t // TODO: use cbor_raw_iterator_next_t, maybe at the cost of an extra local mutable variable
@@ -671,27 +603,6 @@ fn cbor_raw_iterator_next
     }
   }
 }
-
-inline_for_extraction
-let cbor_raw_iterator_truncate_t
-  (#elt_high #cbor_raw_iterator: Type0)
-  (cbor_raw_iterator_match: perm -> cbor_raw_iterator -> list elt_high -> slprop)
-=
-  (c: cbor_raw_iterator) ->
-  (len: U64.t) ->
-  (#pm: perm) ->
-  (#r: Ghost.erased (list elt_high)) ->
-  stt cbor_raw_iterator
-  (requires
-    cbor_raw_iterator_match pm c r **
-    pure (U64.v len <= List.Tot.length r)
-  )
-  (ensures fun res ->
-    cbor_raw_iterator_match 1.0R res (fst (List.Tot.splitAt (U64.v len) r)) **
-    Trade.trade
-      (cbor_raw_iterator_match 1.0R res (fst (List.Tot.splitAt (U64.v len) r)))
-      (cbor_raw_iterator_match pm c r)
-  )
 
 inline_for_extraction
 let cbor_raw_serialized_iterator_truncate_t
