src/cbor/pulse/raw/CBOR.Pulse.Raw.Format.Serialized.C.fsti
@@ -1,0 +1,51 @@
+module CBOR.Pulse.Raw.Format.Serialized.C
+open CBOR.Pulse.Raw.Format.Match.C
+open CBOR.Pulse.Raw.Iterator.C
+open CBOR.Spec.Raw.Base
+open Pulse.Lib.Pervasives
+open Pulse.Lib.Trade
+
+module PM = Pulse.Lib.SeqMatch
+module A = Pulse.Lib.Array
+module S = Pulse.Lib.Slice
+module R = Pulse.Lib.Reference
+module SZ = FStar.SizeT
+module U64 = FStar.UInt64
+
+val cbor_serialized_array_iterator_match
+  (p: perm)
+  (i: cbor_raw_serialized_iterator)
+  (a: list raw_data_item)
+: slprop
+
+val cbor_serialized_array_iterator_init
+  (c: cbor_serialized)
+  (#pm: perm)
+  (#r: Ghost.erased raw_data_item { Array? r })
+: stt cbor_raw_serialized_iterator
+    (cbor_match_serialized_array c pm r)
+    (fun res -> exists* p .
+      cbor_serialized_array_iterator_match p res (Array?.v r) **
+      trade
+        (cbor_serialized_array_iterator_match p res (Array?.v r))
+        (cbor_match_serialized_array c pm r)
+    )
+
+val cbor_serialized_map_iterator_match
+  (p: perm)
+  (i: cbor_raw_serialized_iterator)
+  (a: list (raw_data_item & raw_data_item))
+: slprop
+
+val cbor_serialized_map_iterator_init
+  (c: cbor_serialized)
+  (#pm: perm)
+  (#r: Ghost.erased raw_data_item { Map? r })
+: stt cbor_raw_serialized_iterator
+    (cbor_match_serialized_map c pm r)
+    (fun res -> exists* p .
+      cbor_serialized_map_iterator_match p res (Map?.v r) **
+      trade
+        (cbor_serialized_map_iterator_match p res (Map?.v r))
+        (cbor_match_serialized_map c pm r)
+    )
