src/cbor/pulse/raw/CBOR.Pulse.Raw.Iterator.Gen.fst
@@ -1,0 +1,142 @@
+module CBOR.Pulse.Raw.Iterator.Gen
+open CBOR.Pulse.Raw.Util
+open Pulse.Lib.Pervasives
+open Pulse.Lib.Trade
+
+module PM = Pulse.Lib.SeqMatch.Util
+module S = Pulse.Lib.Slice.Util
+module R = Pulse.Lib.Reference
+module SZ = FStar.SizeT
+module Trade = Pulse.Lib.Trade.Util
+module U8 = FStar.UInt8
+module U64 = FStar.UInt64
+module Util = CBOR.Spec.Util
+
+inline_for_extraction
+let cbor_raw_iterator_init_from_slice_t
+  (#cbor_raw_iterator: Type0)
+  (#elt_low #elt_high: Type0)
+  (elt_match: perm -> elt_low -> elt_high -> slprop)
+  (cbor_raw_iterator_match: perm -> cbor_raw_iterator -> list elt_high -> slprop)
+=
+  (a: S.slice elt_low) ->
+  (#pm: perm) ->
+  (#pm': perm) ->
+  (#l: Ghost.erased (list elt_high)) ->
+  (#sq: Ghost.erased (Seq.seq elt_low)) ->
+  stt cbor_raw_iterator
+  (requires
+  pts_to a #pm sq **
+  PM.seq_list_match sq l (elt_match pm') **
+  pure (FStar.UInt.fits (SZ.v (S.len a)) U64.n)
+  )
+  (ensures fun res -> exists* p .
+  cbor_raw_iterator_match p res l **
+     trade
+       (cbor_raw_iterator_match p res l)
+       (pts_to a #pm sq **
+         PM.seq_list_match sq l (elt_match pm')
+       )
+  )
+
+inline_for_extraction
+let cbor_raw_iterator_init_from_serialized_t
+  (#cbor_raw_serialized_iterator #cbor_raw_iterator: Type0)
+  (#elt_high: Type0)
+  (ser_match: perm -> cbor_raw_serialized_iterator -> list elt_high -> slprop)
+  (cbor_raw_iterator_match: perm -> cbor_raw_iterator -> list elt_high -> slprop)
+=
+  (a: cbor_raw_serialized_iterator) ->
+  (#pm: perm) ->
+  (#l: Ghost.erased (list elt_high)) ->
+  stt cbor_raw_iterator
+  (requires
+  ser_match pm a l
+  )
+  (ensures fun res -> exists* p .
+  cbor_raw_iterator_match p res l **
+     trade
+       (cbor_raw_iterator_match p res l)
+       (ser_match pm a l)
+  )
+
+inline_for_extraction
+let cbor_raw_iterator_is_empty_t
+  (#elt_high #cbor_raw_iterator: Type0)
+  (cbor_raw_iterator_match: perm -> cbor_raw_iterator -> list elt_high -> slprop)
+= (c: cbor_raw_iterator) ->
+  (#pm: perm) ->
+  (#r: Ghost.erased (list elt_high)) ->
+  stt bool
+  (requires
+    cbor_raw_iterator_match pm c r
+  )
+  (ensures fun res ->
+    cbor_raw_iterator_match pm c r **
+    pure (res == Nil? r)
+  )
+
+inline_for_extraction
+let cbor_raw_iterator_length_t
+  (#elt_high #cbor_raw_iterator: Type0)
+  (cbor_raw_iterator_match: perm -> cbor_raw_iterator -> list elt_high -> slprop)
+=
+  (c: cbor_raw_iterator) ->
+  (#pm: perm) ->
+  (#r: Ghost.erased (list elt_high)) ->
+  stt U64.t
+  (requires
+    cbor_raw_iterator_match pm c r
+  )
+  (ensures fun res ->
+    cbor_raw_iterator_match pm c r **
+    pure ((U64.v res <: nat) == List.Tot.length r)
+  )
+
+inline_for_extraction
+let cbor_raw_iterator_next_t
+  (#cbor_raw_iterator: Type0)
+  (#elt_low #elt_high: Type0)
+  (elt_match: perm -> elt_low -> elt_high -> slprop)
+  (cbor_raw_iterator_match: perm -> cbor_raw_iterator -> list elt_high -> slprop)
+=
+  (pi: R.ref (cbor_raw_iterator)) ->
+  (#pm: perm) ->
+  (#i: Ghost.erased cbor_raw_iterator) ->
+  (#l: Ghost.erased (list elt_high)) ->
+  stt elt_low
+  (
+    R.pts_to pi i **
+    cbor_raw_iterator_match pm i l **
+    pure (Cons? l)
+  )
+  (fun res -> exists* a p i' q .
+    elt_match p res a **
+    R.pts_to pi i' **
+    cbor_raw_iterator_match pm i' q **
+    trade
+      (elt_match p res a ** cbor_raw_iterator_match pm i' q)
+      (cbor_raw_iterator_match pm i l) **
+    pure (Ghost.reveal l == a :: q)
+  )
+
+inline_for_extraction
+let cbor_raw_iterator_truncate_t
+  (#elt_high #cbor_raw_iterator: Type0)
+  (cbor_raw_iterator_match: perm -> cbor_raw_iterator -> list elt_high -> slprop)
+=
+  (c: cbor_raw_iterator) ->
+  (len: U64.t) ->
+  (#pm: perm) ->
+  (#r: Ghost.erased (list elt_high)) ->
+  stt cbor_raw_iterator
+  (requires
+    cbor_raw_iterator_match pm c r **
+    pure (U64.v len <= List.Tot.length r)
+  )
+  (ensures fun res ->
+    cbor_raw_iterator_match 1.0R res (fst (List.Tot.splitAt (U64.v len) r)) **
+    Trade.trade
+      (cbor_raw_iterator_match 1.0R res (fst (List.Tot.splitAt (U64.v len) r)))
+      (cbor_raw_iterator_match pm c r)
+  )
